different linking lemmata

theories/c_toy_lang/melocoton/examples.v
@@ -40,6 +40,14 @@ Definition exampleEnv name : prog_environ := {|
     | _ => ⌜False⌝%I end
 |}.
 
+
+Definition exampleEnvAfterLinking name : prog_environ := {|
+  weakestpre.prog := insert "fiba" (fib_func "fib") (exampleProgram name);
+  T := λ s v Φ, match (s,v) with
+    | ("store_it", [ #(LitLoc l) ; v' ]) => (∃ v, (l I↦ v) ∗ ((l ↦{DfracOwn 1} v') -∗ Φ (#0)))%I
+    | _ => ⌜False⌝%I end
+|}.
+
 (* A simple recursive function *)
 
 Lemma fib_prog_correct (n:nat)
@@ -85,7 +93,7 @@ Proof.
     assert (n = S (S (n-2))) as -> by lia.
     cbn. do 2 f_equal. lia.
 Qed.
-Opaque fib.
+
 Lemma heap_prog_correct (n:nat)
   : ⊢ (WP heap_example @ exampleEnv "fib"; ⊤ {{ v, ⌜v = #(1337 + fib 3)⌝ }}).
 Proof.
@@ -110,5 +118,105 @@ Proof.
   wp_pures.
   done.
 Qed.
+
+  Section linking.
+
+  (* This section is very ugly *)
+  (* Ugly tactic to reduce matches on strings *)
+  Ltac string_resolve s := 
+      repeat (destruct s as [|[[] [] [] [] [] [] [] []] s]; try congruence; eauto).
+
+
+
+  (* Lemma using the "recursive link" lemma*)
+  Lemma fiba_correct_link_rec (n:nat)
+    : ⊢ (WP (call: &"fib" with (Val #n)) @ exampleEnvAfterLinking "fiba"; ⊤ {{ v, ⌜v = #(fib n)⌝ }}).
+  Proof.
+    iStartProof.
+    iApply (wp_link_rec (exampleEnv "fiba") _ _ "fiba").
+    2: iPureIntro; cbn; reflexivity.
+    1: iPureIntro; cbn; unfold exampleEnv, exampleProgram; set_solver.
+    - iIntros "!> %s %vv %Ψ [%Hdom %Hne] HT".
+      unfold exampleEnv, exampleEnvAfterLinking; cbn.
+      string_resolve s. (* <- Takes some time *)
+    - (* We now need to show that the successor state of the function call we are replacing,
+         within the old/smaller context. We have already proven this. Unfortunately, we have not proven
+         such that we can use it here, so we repeat the proof *)
+      iIntros "!> %vv %Ψ HT"; destruct vv as [|[[]] []]; cbn -[apply_func]; eauto.
+      iDestruct "HT" as "(%HTL & HT)". clear n. assert (exists n:nat, Z.of_nat n = n0) as (n & <-).
+      1: exists (Z.to_nat n0); lia. 
+      clear HTL. cbn. wp_finish.
+    { (* From here, we mostly copy from the fib_prog_correct code above *)
+    iStartProof.
+    wp_pures.
+    destruct (bool_decide _) eqn:Heq.
+    - wp_pures. iModIntro. apply bool_decide_eq_true in Heq.
+      assert (n=0 \/ n=1) as [-> | ->] by lia; done.
+    - do 2 wp_pure _. apply bool_decide_eq_false in Heq. wp_bind (FunCall _ _).
+      wp_apply wp_wand.
+      { assert ((n-1)%Z=(n-1)%nat) as -> by lia. iApply (fiba_prog_correct (n-1)). }
+      iIntros (v) "->". wp_bind (FunCall _ _). wp_pure _. wp_apply wp_wand.
+      { assert ((n-2)%Z=(n-2)%nat) as -> by lia. iApply (fiba_prog_correct (n-2)). }
+      iIntros (v) "->". wp_pures. iModIntro. rewrite <- Nat2Z.inj_add. rewrite Nat2Z.id.
+      assert (n = S (S (n-2))) as -> by lia. cbn.
+      assert (n-2-0=n-2) as -> by lia. iApply "HT".
+    }
+    - iApply fiba_prog_correct.
+  Qed.
+
+  (* We now do the same with the other linking lemma, where we must show that the implementation of
+     the function we are replacing is correct, and not the "successor state after function invokation".
+     The flipside is that we have to do this proof in the new environment. 
+
+     In that environment, fib and fiba are mutually recursive, so we have to redo the entire correctness proof. *)
+  Lemma fiba_prog_correct_for_link (n:nat)
+    : ⊢ ((WP (call: &"fib" with (Val #n)) @ exampleEnvAfterLinking "fiba"; ⊤ {{ v, ⌜v = #(fib n)⌝ }}) ∗
+         WP (call: &"fiba" with (Val #n)) @ exampleEnvAfterLinking "fiba"; ⊤ {{ v, ⌜v = #(fib n)⌝ }}).
+  Proof.
+    iStartProof.
+    iLöb as "IH" forall (n). iSplitL.
+    all: wp_pures.
+    all: destruct (bool_decide _) eqn:Heq.
+    1,3: wp_pures; iModIntro; apply bool_decide_eq_true in Heq.
+    1,2:  assert (n=0 \/ n=1) as [-> | ->] by lia; done.
+    all: do 2 wp_pure _; apply bool_decide_eq_false in Heq; wp_bind (FunCall _ _).
+    all: wp_apply wp_wand.
+    1,3: assert ((n-1)%Z=(n-1)%nat) as -> by lia.
+    1,2: iDestruct ("IH" $! _) as "(IH1 & IH2)". 1: iApply "IH2". 1: iApply "IH1".
+    all: iIntros (v) "->"; wp_bind (FunCall _ _); wp_pure _; wp_apply wp_wand.
+    1,3: assert ((n-2)%Z=(n-2)%nat) as -> by lia.
+    1,2: iDestruct ("IH" $! _) as "(IH1 & IH2)". 1: iApply "IH2". 1: iApply "IH1".
+    all: iIntros (v) "->"; wp_pures; iModIntro; iPureIntro; rewrite <- Nat2Z.inj_add.
+    all: repeat f_equal.
+    all: assert (n = S (S (n-2))) as -> by lia.
+    all: cbn; do 2 f_equal; lia.
+  Qed.
+  Opaque fib.
+
+  (* we can now use this result above to prove the linking. Note that we have not actually gained anything,
+     our linking proof presupposes a proof that the entire program is correct all on its own *)
+
+  Lemma fiba_correct_link (n:nat)
+    : ⊢ (WP (call: &"fib" with (Val #n)) @ exampleEnvAfterLinking "fiba"; ⊤ {{ v, ⌜v = #(fib n)⌝ }}).
+  Proof.
+    iStartProof.
+    iApply (wp_link (exampleEnv "fiba") _ _ "fiba").
+    2: iPureIntro; cbn; reflexivity.
+    1: iPureIntro; cbn; unfold exampleEnv, exampleProgram; set_solver.
+    - iIntros "!> %s %vv %Ψ [%Hdom %Hne] HT".
+      unfold exampleEnv, exampleEnvAfterLinking; cbn.
+      string_resolve s.
+    - iIntros "!> %vv %Ψ HT"; destruct vv as [|[[]] []]; cbn; eauto.
+      iDestruct "HT" as "(%HTL & HT)". clear n. assert (exists n:nat, Z.of_nat n = n0) as (n & <-).
+      1: exists (Z.to_nat n0); lia.
+      wp_apply wp_wand.
+      {iDestruct (fiba_prog_correct_for_link _) as "(H1 & H2)". iApply "H2". }
+      iIntros (v) "->". by rewrite Nat2Z.id.
+    - iApply fiba_prog_correct.
+  Qed.
+
+
+  End linking.
+
 
 End examples.
